simplified the SBpass design   1) at the beginning of a function, always allocates two slots for loading metadata of pointers from memory, so we do not need to prove that it is safe to ignore them when there are no pointer-loading in the function.   2) We had a problem about proving malloc does not change constant values. The case is like this    suppose the original code is      %1 = malloc typ, i32 const ;; here const is the size to allocate,    if the instrumentation is      %1 = malloc typ, i32 const      %base = %1      %bound gep %1, i32 const    we need to argument that the value represented by const is the 'same' before and after this malloc, which is obvious, but needs some work.    Currently, we transformed it by      %tmp = bitcast i32 cosnt to i32      %1 = malloc typ, i32 %tmp      %base = %1      %bound gep %1, i32 %tmp    Now the result is trivial, since registered values are unchanged for sure.   3) decomposed the dependency with sb_db_trans.v, which will be removed when sb_ds_trans is proved.   4) The requirememt of shadow-stack:
caller pushes normal base/bound for ptr parameters, but, rather than
skipping nptr parameters, also pushes null/null for them.
 for example, if a caller thinks a call has signature
     i8 %1 = foo (i8* a) (i8 b) (i8* c)
 it does
     allocate_ss (1 + 3) // 1 for ret, 3 for parameters
     set_ss_basebound a_metadata 1
     set_ss_basebound null 2
     set_ss_basebound c_metadata 3
     call foo...
     deallocate_ss

If the allocate_ss always zero-outs allocated shadow-stack, caller does
not need to push null/null additionally.

callee pops ptr argument's metadata w.r.t its index (the index of the
whole arg lists, not only args with ptr typs)
 e.g. if a call has signature
      %1 foo (i8 a) (i8* b) (i8* c) { .. }
 it does, at its beginning
     b_metadata = get_ss_basebound 2
     c_metadata = get_ss_basebound 3

 If callee wants to pop more than caller pushs, it returns null/null
 the default metadata for return is null/null in the case caller sets
nothing to its return.

To make the wrapper just work (for the program with matched function types), 
We simply changed in softbound.c @ main to be

__softboundcetswithss_allocate_shadow_stack_space(3);   // from 2 to 3
__softboundcetswithss_store_base_shadow_stack(NULL, 1); // added
__softboundcetswithss_store_bound_shadow_stack(NULL, 1); // added
__softboundcetswithss_store_base_shadow_stack(&new_argv[0], 2); // 1 to 2
__softboundcetswithss_store_bound_shadow_stack(temp_ptr, 2); // 1 to 2
return_value = softbound_pseudo_main(argc, new_argv);
__softboundcetswithss_deallocate_shadow_stack_space();

All existing wrappers only have ptr args as its first argument, so we do not 
need to change them. But if not so, we need to ensure indices are
matched.



git-svn-id: https://webdav.seas.upenn.edu/svn/sol/vol@3001 eef5ea85-cc2e-0410-bd84-0fae1f012da8

src/SoftBound/sb_ds_def.v
@@ -40,35 +40,34 @@ Definition base2GV := blk2GV.
 Definition bound2GV (TD:TargetData) (b:mblock) (s:sz) n : GenericValue :=
 ptr2GV TD (Vptr b (Int.repr 31 ((Size.to_Z s)*n))).
 
-Fixpoint get_const_metadata (c:const) : option (const*const*typ) :=
+Fixpoint get_const_metadata (c:const) : option (const*const) :=
 match c with
 | const_gid t gid => 
     match t with
-    | typ_function _ _ _ => Some (c, c, (typ_pointer t))
+    | typ_function _ _ _ => Some (c, c)
     | _ => Some (c, const_gep false c 
              (Cons_list_const (const_int Size.ThirtyTwo 
-               (INTEGER.of_Z 32%Z 1%Z false)) Nil_list_const), (typ_pointer t))
+               (INTEGER.of_Z 32%Z 1%Z false)) Nil_list_const))
     end
 | const_gep _ pc _ => get_const_metadata pc
 | const_castop castop_bitcast pc (typ_pointer _) => get_const_metadata pc
 | _ => None
 end.
 
-Definition get_reg_metadata TD M gl (rm:rmetadata) (v:value) 
-    : option (metadata * typ) :=
+Definition get_reg_metadata TD M gl (rm:rmetadata) (v:value) : option metadata :=
   match v with
   | value_id pid => 
       match lookupAL _ rm pid with
-      | Some md => Some (md, typ_pointer (typ_int Size.Eight))
+      | Some md => Some md
       | _ => None
       end
   | value_const c => 
       match get_const_metadata c with
-      | Some (bc, ec, t) => 
+      | Some (bc, ec) => 
           do gvb <- const2GV TD M gl bc;
           do gve <- const2GV TD M gl ec;
-          ret (mkMD gvb gve, t)
-      | None => Some (mkMD null null, typ_pointer (typ_int Size.Eight))
+          ret (mkMD gvb gve)
+      | None => Some (mkMD null null)
       end
   end.
 
@@ -147,7 +146,7 @@ Mmap               : mmetadata
 
 Fixpoint getIncomingValuesForBlockFromPHINodes (TD:TargetData) (M:mem) 
   (PNs:list phinode) (b:block) (gl lc:GVMap) (rm:rmetadata) : 
-  option (list (id * GenericValue * option (metadata*typ))) :=
+  option (list (id * GenericValue * option metadata)) :=
 match PNs with
 | nil => Some nil
 | (insn_phi id0 t vls)::PNs => 
@@ -160,7 +159,7 @@ match PNs with
       | (Some gv1, Some idgvs) => 
           if isPointerTypB t then
             match get_reg_metadata TD M gl rm v with
-            | Some (md,mt) => Some ((id0,gv1,Some (md,mt))::idgvs)
+            | Some md => Some ((id0,gv1,Some md)::idgvs)
             | None => None
             end
           else Some ((id0,gv1,None)::idgvs)
@@ -170,7 +169,7 @@ match PNs with
 end.
 
 Fixpoint updateValuesForNewBlock 
-  (ResultValues:list (id*GenericValue*option (metadata*typ))) (lc:GVMap) 
+  (ResultValues:list (id*GenericValue*option metadata)) (lc:GVMap) 
   (rm:rmetadata) : GVMap * rmetadata :=
 match ResultValues with
 | nil => (lc, rm)
@@ -178,7 +177,7 @@ match ResultValues with
     let '(lc', rm') := updateValuesForNewBlock ResultValues' lc rm in
     match opmd with
     | None => (updateAddAL _ lc' id0 v, rm')
-    | Some (md,_) => prop_reg_metadata lc' rm' id0 v md
+    | Some md => prop_reg_metadata lc' rm' id0 v md
     end
 end.
 
@@ -221,7 +220,7 @@ Definition returnUpdateLocals (TD:TargetData) (M:mem) (c':cmd)
             match t with
             | typ_function (typ_pointer _) _ _ =>
               match get_reg_metadata TD M gl rm Result with
-              | Some (md,_) => Some (prop_reg_metadata lc' rm' id0 gr md)
+              | Some md => Some (prop_reg_metadata lc' rm' id0 gr md)
               | None => Some 
                   (prop_reg_metadata lc' rm' id0 gr (mkMD null null))
               end
@@ -251,7 +250,7 @@ Definition exCallUpdateLocals (ft:typ) (noret:bool) (rid:id)
   end.
 
 Fixpoint params2GVs (TD:TargetData) (M:mem) (lp:params) (lc gl:GVMap) 
- (rm:rmetadata) : option (list (GenericValue * option (metadata*typ))) :=
+ (rm:rmetadata) : option (list (GenericValue * option metadata)) :=
 match lp with
 | nil => Some nil
 | (t, v)::lp' => 
@@ -264,7 +263,7 @@ match lp with
 end.
 
 Fixpoint _initializeFrameValues (la:args) 
-  (lg:list (GenericValue*option (metadata*typ))) (lc:GVMap) (rm : rmetadata) 
+  (lg:list (GenericValue*option metadata)) (lc:GVMap) (rm : rmetadata) 
   : GVMap * rmetadata :=
 match (la, lg) with
 | ((t, _, id0)::la', (gv, opmd)::lg') => 
@@ -272,7 +271,7 @@ match (la, lg) with
      if isPointerTypB t then
        match opmd with
        | None => (prop_reg_metadata lc' rm' id0 gv (mkMD null null))
-       | Some (md,_) => (prop_reg_metadata lc' rm' id0 gv md)
+       | Some md => (prop_reg_metadata lc' rm' id0 gv md)
        end
      else (updateAddAL _ lc' id0 gv, rm')
 | ((t, _, id0)::la', nil) => 
@@ -283,7 +282,7 @@ match (la, lg) with
 | _ => (lc, rm)
 end.
 
-Definition initLocals (la:args) (lg:list (GenericValue*option (metadata*typ))) 
+Definition initLocals (la:args) (lg:list (GenericValue*option metadata)) 
   (rm : rmetadata) : GVMap * rmetadata :=
 _initializeFrameValues la lg nil rm.
 
@@ -434,8 +433,8 @@ Inductive dsInsn : State -> State -> trace -> Prop :=
     trace_nil
 
 | dsLoad_nptr : forall S TD Ps F B lc rm gl fs id t align vp EC cs tmn Mem als 
-    gvp gv MM md mt,
-  get_reg_metadata TD Mem gl rm vp = Some (md,mt) ->
+    gvp gv MM md,
+  get_reg_metadata TD Mem gl rm vp = Some md ->
   getOperandValue TD Mem vp lc gl = Some gvp ->
   assert_mptr TD t gvp md ->
   mload TD Mem gvp t align = Some gv ->
@@ -449,8 +448,8 @@ Inductive dsInsn : State -> State -> trace -> Prop :=
     trace_nil
 
 | dsLoad_ptr : forall S TD Ps F B lc rm gl fs id t align vp EC cs tmn Mem MM als 
-    gvp gv md md' lc' rm' mt,
-  get_reg_metadata TD Mem gl rm vp = Some (md,mt) ->
+    gvp gv md md' lc' rm',
+  get_reg_metadata TD Mem gl rm vp = Some md ->
   getOperandValue TD Mem vp lc gl = Some gvp ->
   assert_mptr TD t gvp md ->
   mload TD Mem gvp t align = Some gv ->
@@ -465,8 +464,8 @@ Inductive dsInsn : State -> State -> trace -> Prop :=
     trace_nil
 
 | dsStore_nptr : forall S TD Ps F B lc rm gl fs sid t align v vp EC cs tmn Mem MM
-    als gv gvp md Mem' mt,
-  get_reg_metadata TD Mem gl rm vp = Some (md,mt) ->
+    als gv gvp md Mem',
+  get_reg_metadata TD Mem gl rm vp = Some md ->
   getOperandValue TD Mem v lc gl = Some gv ->
   getOperandValue TD Mem vp lc gl = Some gvp ->
   assert_mptr TD t gvp md ->
@@ -481,14 +480,14 @@ Inductive dsInsn : State -> State -> trace -> Prop :=
     trace_nil
 
 | dsStore_ptr : forall S TD Ps F B lc rm gl fs sid t align v vp EC cs tmn Mem MM
-    als gv gvp md md' Mem' MM' mt mt',
-  get_reg_metadata TD Mem gl rm vp = Some (md,mt) ->
+    als gv gvp md md' Mem' MM',
+  get_reg_metadata TD Mem gl rm vp = Some md ->
   getOperandValue TD Mem v lc gl = Some gv ->
   getOperandValue TD Mem vp lc gl = Some gvp ->
   assert_mptr TD t gvp md ->
   mstore TD Mem gvp t gv align = Some Mem' ->
   isPointerTypB t = true ->
-  get_reg_metadata TD Mem gl rm v = Some (md',mt') ->
+  get_reg_metadata TD Mem gl rm v = Some md' ->
   set_mem_metadata TD MM gvp md' = MM' -> 
   dsInsn 
     (mkState S TD Ps 
@@ -499,8 +498,8 @@ Inductive dsInsn : State -> State -> trace -> Prop :=
     trace_nil
 
 | dsGEP : forall S TD Ps F B lc rm gl fs id inbounds t vp idxs vidxs EC gvp gvp' 
-                 cs tmn Mem MM als lc' rm' md mt,
-  get_reg_metadata TD Mem gl rm vp = Some (md,mt) ->
+                 cs tmn Mem MM als lc' rm' md,
+  get_reg_metadata TD Mem gl rm vp = Some md ->
   getOperandValue TD Mem vp lc gl = Some gvp ->
   values2GVs TD Mem idxs lc gl = Some vidxs ->
   GEP TD t gvp vidxs inbounds = Some gvp' ->
@@ -548,10 +547,10 @@ Inductive dsInsn : State -> State -> trace -> Prop :=
     trace_nil
 
 | dsBitcast_ptr : forall S TD Ps F B lc rm gl fs id t1 v1 t2 gv2 EC cs tmn Mem MM
-    als md lc' rm' mt,
+    als md lc' rm',
   CAST TD Mem lc gl castop_bitcast t1 v1 t2 = Some gv2 ->
   isPointerTypB t1 = true ->
-  get_reg_metadata TD Mem gl rm v1 = Some (md,mt) ->
+  get_reg_metadata TD Mem gl rm v1 = Some md ->
   prop_reg_metadata lc rm id gv2 md = (lc', rm') ->
   dsInsn 
     (mkState S TD Ps 
@@ -625,13 +624,13 @@ Inductive dsInsn : State -> State -> trace -> Prop :=
     trace_nil
 
 | dsSelect_ptr : forall S TD Ps F B lc rm gl fs id v0 t v1 v2 c EC cs tmn Mem MM
-    als gv1 gv2 md1 md2 lc' rm' mt1 mt2,
+    als gv1 gv2 md1 md2 lc' rm',
   getOperandValue TD Mem v0 lc gl = Some c ->
   getOperandValue TD Mem v1 lc gl = Some gv1 ->
   getOperandValue TD Mem v2 lc gl = Some gv2 ->
   isPointerTypB t = true ->
-  get_reg_metadata TD Mem gl rm v1 = Some (md1,mt1) ->
-  get_reg_metadata TD Mem gl rm v2 = Some (md2,mt2) ->
+  get_reg_metadata TD Mem gl rm v1 = Some md1 ->
+  get_reg_metadata TD Mem gl rm v2 = Some md2 ->
   (if isGVZero TD c then 
     prop_reg_metadata lc rm id gv2 md2
   else
